clib: add a `hoarep_rewrite` method
This is like `ccorres_rewrite`, but for `hoarep`, and uses the same
infrastructure.

The interaction between the `simpl_rewrite` locale and the
`simpl_rewrite` method was confusing, and didn't work well with multiple
interpretations. We replace the locale with a simple anonymous context
block. Since that puts more things in the global namespace, we rename
many of them. The `simpl_rewrite` method is now parameterised by a `hom`
fact which determines the predicate under which we are rewriting.

This also includes a slight generalisation of `exec_eq_is_valid_eq`,
which allows a similar generalisation of `hoarep_rewrite`.

Signed-off-by: Matthew Brecknell <Matthew.Brecknell@data61.csiro.au>

lib/clib/CCorres_Rewrite.thy
@@ -8,40 +8,48 @@ theory CCorres_Rewrite
 imports Corres_UL_C Simpl_Rewrite
 begin
 
-text \<open>A simple proof method for rewriting Simpl programs under @{term ccorres_underlying}.\<close>
+text \<open>Simple proof methods for rewriting Simpl programs under @{term ccorres_underlying}
+      and @{term hoarep}.\<close>
 
-locale ccorres_rewrite_locale =
-  simpl_rewrite \<Gamma> "ccorres_underlying sr \<Gamma> r xf r' xf' P P' hs H"
-  for \<Gamma> sr r xf r' xf' P P' hs H
-
-global_interpretation ccorres_rewrite: ccorres_rewrite_locale
-  by unfold_locales (auto simp: simpl_rewrite_base.com_eq_def semantic_equiv_def ceqv_def
-                          elim: ccorres_semantic_equivD2)
+lemma ccorres_com_eq_hom:
+  "com_eq_hom \<Gamma> (ccorres_underlying sr \<Gamma> r xf r' xf' P P' hs H)"
+  by (auto simp: com_eq_hom_def com_eq_def semantic_equiv_def ceqv_def
+           elim: ccorres_semantic_equivD2)
 
 method ccorres_rewrite declares C_simp C_simp_pre C_simp_simps C_simp_throws
-  = ccorres_rewrite.simpl_rewrite
+  = simpl_rewrite hom: ccorres_com_eq_hom
 
-abbreviation "com_eq \<Gamma> \<equiv> ccorres_rewrite.com_eq \<Gamma> True"
-abbreviation "never_continues \<Gamma> \<equiv> ccorres_rewrite.never_continues \<Gamma> True"
+lemma hoarep_com_eq_hom:
+  "com_eq_hom \<Gamma> (\<lambda>c. hoarep \<Gamma> {} F P c Q A)"
+  by (auto simp: com_eq_hom_def com_eq_def ceqv_def
+           elim: exec_eq_is_valid_eq0[rotated])
 
-lemmas com_eq_def = ccorres_rewrite.com_eq_def
-lemmas never_continues_def = ccorres_rewrite.never_continues_def
+lemma hoarep_spec_com_eq_hom:
+  "com_eq_hom \<Gamma> (\<lambda>c. \<forall>s. hoarep \<Gamma> {} (F s) (P s) c (Q s) (A s))"
+  by (fastforce simp: com_eq_hom_def com_eq_def ceqv_def
+                elim: exec_eq_is_valid_eq0[rotated])
+
+method hoarep_rewrite declares C_simp C_simp_pre C_simp_simps C_simp_throws
+  = (match conclusion in \<open>hoarep \<Gamma> {} F P c Q A\<close> for \<Gamma> F P c Q A
+                           \<Rightarrow> \<open>simpl_rewrite hom: hoarep_com_eq_hom\<close>
+                       \<bar> \<open>\<forall>s. hoarep \<Gamma> {} (F s) (P s) c (Q s) (A s)\<close> for \<Gamma> F P c Q A
+                           \<Rightarrow> \<open>simpl_rewrite hom: hoarep_spec_com_eq_hom\<close>)
 
 text \<open>Some CRefine proofs remove Collect_const from the @{method simp} set,
       but we almost always want @{method ccorres_rewrite} to use it to simplify
       trivial @{text IF} and @{text WHILE} conditions.\<close>
 declare Collect_const [C_simp_simps]
 
-text \<open>Test that the @{command named_theorems} @{thm C_simp} still works in the
-      @{term ccorres_rewrite_locale} interpretation.\<close>
+text \<open>Test\<close>
 
 lemma
-  assumes c3: "com_eq \<Gamma> c3 c"
-  assumes c: "com_eq \<Gamma> (c;;c) c"
+  assumes c3: "com_equiv \<Gamma> c3 c"
+  assumes c: "com_equiv \<Gamma> (c;;c) c"
   shows "ccorres_underlying sr \<Gamma> r xf r' xf' P P' hs H
                             (c;; Guard f UNIV (IF X THEN c ELSE c FI);; Cond {} Skip (Skip;;c2);;
                              Skip;;
                              (IF False THEN Skip ELSE SKIP;; TRY THROW CATCH c3 END FI;; SKIP))"
+  supply Collect_const[simp del]
   apply ccorres_rewrite
   apply (match conclusion in "ccorres_underlying sr \<Gamma> r xf r' xf' P P' hs H (c;;c;;c2;;c3)" \<Rightarrow> \<open>-\<close>)
   apply (ccorres_rewrite C_simp: c3)
